instantiation/LoadData.thy
@@ -699,7 +699,7 @@ qed
 theorem SemanticsLoadData:
   assumes prov: "LoadDataAction auth a l \<in> actions"
       and valid: "getStateIsValid s"
-      and suc: "(PreserveDomain actions, s') \<in> NextStates s"
+      and suc: "(PreserveDomain actions, s') \<in> SemanticsCheriMips s"
   shows "Permit_Load (getPerms (getCapReg auth s))"
         "getTag (getCapReg auth s)"
         "\<not> getSealed (getCapReg auth s)"
@@ -716,11 +716,11 @@ using SemanticsLoadData_NextWithGhostState
 unfolding AddressIsDataReadable_def 
 unfolding getTranslateAddrFunc_def getTranslateAddresses_def
 unfolding StateIsValid_def
-unfolding NextStates_def Next_NextWithGhostState NextNonExceptionStep_def
+unfolding SemanticsCheriMips_def Next_NextWithGhostState NextNonExceptionStep_def
 by (auto simp: ValueAndStatePart_simp split: if_splits option.splits)
 
 corollary LoadDataInstantiation:
-  assumes "(lbl, s') \<in> NextStates s"
+  assumes "(lbl, s') \<in> SemanticsCheriMips s"
   shows "LoadDataProp s lbl s'"
 unfolding LoadDataProp_def
 using assms SemanticsLoadData
