instantiation/SealCap.thy
@@ -114,7 +114,7 @@ theorem SemanticsSealCap:
   fixes s auth
   defines "t \<equiv> ucast (getBase (getCapReg auth s)) + ucast (getOffset (getCapReg auth s))"
   assumes prov: "SealCapAction auth cd cd' \<in> actions"
-      and suc: "(PreserveDomain actions, s') \<in> NextStates s"
+      and suc: "(PreserveDomain actions, s') \<in> SemanticsCheriMips s"
   shows "Permit_Seal (getPerms (getCapReg auth s))"
         "getTag (getCapReg auth s)"
         "\<not> getSealed (getCapReg auth s)"
@@ -129,11 +129,11 @@ using SemanticsSeal_NextWithGhostState
                 authAccessible="getRegisterIsAccessible auth s",
           THEN HoareTripleE[where s=s]]
 unfolding t_def SemanticsSealPost_def Let_def
-unfolding NextStates_def Next_NextWithGhostState NextNonExceptionStep_def
+unfolding SemanticsCheriMips_def Next_NextWithGhostState NextNonExceptionStep_def
 by (auto simp: ValueAndStatePart_simp split: if_splits option.splits)
 
 corollary SealCapInstantiation:
-  assumes "(lbl, s') \<in> NextStates s"
+  assumes "(lbl, s') \<in> SemanticsCheriMips s"
   shows "SealCapProp s lbl s'"
 unfolding SealCapProp_def
 using assms SemanticsSealCap
